# Folding Lists - Chapter 10

- [Folding Lists - Chapter 10](#folding-lists-chapter-10)
    - [01](#anchor-01)
    - [02](#anchor-02)
    - [03](#anchor-03)
    - [04](#anchor-04)
    - [05](#anchor-05)
      - [a](#a)
      - [b](#b)
      - [c](#c)
      - [d](#d)
      - [e](#e)
      - [f](#f)
      - [g](#g)
      - [h](#h)
      - [i](#i)
  - [Exercises: Database processing](#exercises-database-processing)
  - [Scans exercises](#scans-exercises)
  - [Warm-up and review](#warm-up-and-review)
    - [01](#anchor-01-1)
    - [02](#anchor-02-1)
    - [03](#anchor-03-1)
    - [Old Versions](#old-versions)
    - [The End](#the-end)

Page 365.

### 01

B and C are correct. Both `foldr` and `foldl` will do because `(*)` is associative. Flipping `(*)` doesnâ€™t change the results, again, because `(*)` is associative.

### 02

```
foldl * 1 [1, 2, 3]

foldl (flip (*)) 1 [1, 2, 3]

foldl (flip (*)) (flip (*) 1 1) [2, 3]

foldl (flip (*)) (flip (*) 1 1) [2, 3]

foldl (flip (*)) ((flip (*)) ((flip (*)) 1 1) 2) [3]

foldl (flip (*)) ((flip (*)) ((flip (*)) ((flip (*)) 1 1) 2) 3) []

((flip (*)) ((flip (*)) ((flip (*)) 1 1) 2) 3)

((flip (*)) ((flip (*)) 1 2) 3)

((flip (*)) 2 3

6
```

Another approach:

```
foldl :: (acc -> x -> acc) -> acc -> [x] -> acc
foldl f z []     = z
foldl f z (x:xs) = foldl f (f z x) xs

f = (*)

foldl (flip f) ((flip f) 1 1) [2, 3]
acc = 1, (1 * 1)

foldl (flip f) ((flip f) 1 2) [3]
acc = 2, (1 * 2)

foldl (flip f) ((flip f) 2 3) []
acc = 6, (2 * 3)

Reaches base case, returns â€˜zâ€™, our â€˜accâ€™.
```

Or, assigning `flip (*)` to a simpler variable to reduce number of parentheses:

```
f = flip (*)

foldl f 1 [1, 2, 3]
foldl f (f 1 1) [2, 3]
           1 (1 * 1 is 1)
foldl f (f 1 2) [3]
           2 (1 * 2 is 2)
foldl f (f 2 3) []
           6 (2 * 3 is 6)
6
```

### 03

C is correct.

### 04

A is correct.

### 05

#### a

Missing the â€œzeroâ€, default, accumulator parameter.

Correct:

```ghci
Î»> foldr (++) [] ["woot", "WOOT", "woot"]
"wootWOOTwoot"
```

#### b

Need a list of strings, not a single string.

Correct:

```ghci
Î»> foldr max [] ["fear", "is", "little", "death"]
"little"
```

#### c

There is no â€œandâ€ function.

Correct:

```haskell
foldr (&&) True [False, True]
```

#### d

It always returns `True`, which is incorrect. We must make the zero produce `False` instead.

```haskell
foldr (||) False [False, True]
```

#### e

```ghci
Î»> foldr ((++) . show) "" [1..5]
"12345"
```

Or flipping `((++) . show)`, although the result is in reverse order:

```GHCi
Î»> foldl (flip ((++) . show)) "" [1, 2, 3]
"321"
```

`foldr` applies `f x` first, so we apply `((++) . show)`to `1` first, converting it to a string, which is `(++)` concatenated to the â€œrest of the foldâ€.

`foldl` applies `f` to the zero/acc first, which *is* a string already, and then tries to `(++)`concatenate it with the number which was *not* converted to a string. It blows up! ðŸ’£

```
Î»> ((++) . show) 1 ""
"1"

Î»> ((++) . show) "" 1
ðŸ’¥ error
```

#### f

Zero has the type â€˜Charâ€™, and the list is of type â€˜Numâ€™. The type of zero and the elements of the list must be the same. Possible solutions, depending on the result sought:

```ghci
Î»> foldr (flip const) 'a' [1, 2, 3]
'a'

Î»> foldl const 'a' [1, 2, 3]
'a'

Î»> foldr const 'a' "bcd"
'b'

Î»> foldr const 'a' ['b', 'c', 'd']
'b'

Î»> foldr const 0 [1, 2, 3]
1
```

#### g

`foldr const 0 "tacos"` is incorrect because the accumulator char `'t'` does not match the type of 0 (the number zero). Possible solutions depending on the result sought:

```ghci
Î»> foldl const 0 "tacos"
0

Î»> foldr (flip const) 0 "tacos"
0

Î»> foldl const "" "tacos"
```

#### h

```ghci
Î»> foldr (flip const) 0 "burritos"
0

Î»> foldl const 0 "burritos"
0
```

#### i

```ghci
Î»> foldr (flip const) 'z' [1..5]
'z'

Î»> foldl const 'z' [1..5]
'z'
```

## Exercises: Database processing

Page 371.

```haskell
{-# LANGUAGE NoMonomorphismRestriction #-}

import Text.Pretty.Simple (pPrint)
import Data.Time

pp = pPrint

data DBItem = DBString String
            | DBNumber Integer
            | DBDate UTCTime
            deriving (Eq, Ord, Show)
theDb :: [] DBItem
theDb =
  [ DBDate (UTCTime (fromGregorian 1911 5 1)
                    (secondsToDiffTime 34123))
  , DBNumber 9001
  , DBString "Hello, World!"
  , DBDate (UTCTime (fromGregorian 1921 5 1)
                    (secondsToDiffTime 34123))
  , DBNumber 100
 ]

filterDbDate :: [] DBItem -> [] UTCTime
filterDbDate items = foldr f [] items
  where
    --   (a     -> b           -> b)
    f :: DBItem -> [] UTCTime -> [] UTCTime
    f (DBDate x) acc = (:) x acc
    f _          acc = acc
--
-- Î»> pp (filterDbDate theDb)
-- [ 1911 - 05 - 01 09 : 28 : 43 UTC
-- , 1921 - 05 - 01 09 : 28 : 43 UTC
-- ]
--
-- `foldr` passes one `DBItem` at a time to the folding function `f`.
--

filterDbNumber :: [] DBItem -> [] Integer
filterDbNumber items = foldr f [] items
  where
    --   (a     -> b           -> b)
    f :: DBItem -> [] Integer -> [] Integer
    f (DBNumber n) nums = (:) n nums
    f _            nums = nums
--
-- Î»> pp $ filterDbNumber theDb
-- [ 9001 ]
--
-- `foldr` passes one `DBItem` at a time to the folding function `f`.
--
-- So, we can't return a `[] DBNumber`. We use it to pattern match on the
-- item, but since `DBNumber` is a data constructor (and not a type), we can't
-- use it in type signatures. Pattern matching is for runtime data.
--


mostRecent :: [] DBItem -> UTCTime
mostRecent items = maximum $ filterDbDate items

leastRecent :: [] DBItem -> UTCTime
leastRecent items = minimum $ filterDbDate items

sumDbNumbers :: [DBItem] -> Integer
sumDbNumbers = sum . filterDbNumber

avgDbNums :: [DBItem] -> Double
avgDbNums items = total / count
  where
    count :: Double
    count = fromIntegral . length . filterDbNumber $ items
    total :: Double
    total = fromIntegral . sumDbNumbers $ items
```

## Scans exercises

Page 378.

```haskell
myScanl :: (a -> b -> a) -> a -> [b] -> [a]
myScanl f q ls =
  q : (case ls of
         [] -> []
         x:xs -> myScanl f (f q x) xs)


res1 = myScanl (+) 1 [1..3]


fib :: Word -> Word
fib 0 = 0
fib 1 = 1
fib n = fib (n - 1) + fib (n - 2)


fibs :: [Word]
fibs = 1 : myScanl (+) 1 fibs


fibsN :: Int -> Word
fibsN n = fibs !! n


fibs20first :: [Word]
fibs20first = take 20 fibs

fibs20 :: [Word]
fibs20 = take 20 $ 1 : myScanl (+) 1 fibs20

fibsLT100 :: [Word]
fibsLT100 = takeWhile (< 100) fibs

fact :: Word -> Word
fact 0 = 1
fact n = n * fact (n - 1)


facts :: [Word]
facts = myScanl (*) 1 [1..]

factN :: Int -> Word
factN n = facts !! n
```

## Warm-up and review

Page 378.

### 01

```haskell
stops :: [Char]
stops = "pbtdkg"

vowels :: [Char]
vowels = "aeiou"

-- Produces all possible three-tuples of stop-vowel-stop combinations.
allCombs :: [Char] -> [Char] -> [(Char, Char, Char)]
allCombs ss vs = [(s, v, s) | s <- ss, v <- vs]

-- Checks whether a tuple starts with the given letter.
startsWith :: Char -> (Char, Char, Char) -> Bool
startsWith c (e, _, _) = c == e

startsWithAorP :: (Char, Char, Char) -> Bool
startsWithAorP (x, _, _) = x == 'a' || x == 'p'

nouns :: [[Char]]
nouns = ["jedi", "padawan", "kitten"]

verbs :: [[Char]]
verbs = ["fight", "run", "meow"]

mkNounVerbNoun :: [[Char]] -> [[Char]] -> [([Char], [Char], [Char])]
mkNounVerbNoun ns vs = [(n, v, n) | n <- ns, v <- vs]
```

### 02

Finds the average of the length of the words in the input string.

### 03

```haskell
-- Using â€˜whereâ€™.
avgWordLen :: [Char] -> Double
avgWordLen str = (/) numWordChars lenWords
  where
    numWordChars = fromIntegral $ sum (map length (words str))
    lenWords     = fromIntegral $ length (words str)

-- Using â€˜letâ€™.
avgWordLen :: [Char] -> Double
avgWordLen str =
  let
    numWordChars = fromIntegral $ sum (map length (words str))
    lenWords     = fromIntegral $ length (words str)
  in
    (/) numWordChars lenWords

--
-- Version I come up during 2021 studies of this book.
--
avgWordLen :: String -> Double
avgWordLen s = (/) numChars numWords
  where
    numChars :: Double
    numChars = fromIntegral $ sum $ map length $ words s
    numWords :: Double
    numWords = fromIntegral $ length $ words s
--
-- Î»> avgWordLen "The force is strong with this one. Most impressive!"
-- 4.777777777777778
--
```

----
### Old Versions

```haskell
-- Direct recursion, not using â€˜&&â€™.
myAnd' :: [Bool] -> Bool
myAnd' [] = True
myAnd' (x:xs) =
  if x == False
  then False
  else myAnd xs

-- Direct recursion using â€˜&&â€™.
myAnd'' :: [Bool] -> Bool
myAnd'' [] = True
myAnd'' (x:xs) = x && myAnd' xs

-- Fold, not point-free.
myAnd''' :: [Bool] -> Bool
myAnd''' = foldr f True
  where f = (\x acc ->
               if x == False
               then False
               else acc)

-- Both â€˜myAndâ€™ and the folding function are point-free.
myAnd :: [Bool] -> Bool
myAnd = foldr (&&) True


-- Direct recursion not using â€˜||â€™.
myOr' :: [Bool] -> Bool
myOr' [] = False
myOr' (x:xs) =
  if x == True
  then True
  else myOr' xs

-- Direct recursion using â€˜||â€™.
myOr'' :: [Bool] -> Bool
myOr'' [] = False
myOr'' (x:xs) = x || myOr'' xs

-- Fold, not point-free.
myOr''' :: [Bool] -> Bool
myOr''' = foldr f False
  where f = (\x acc ->
               if x == True
               then True
               else acc)

-- Both â€˜myOrâ€™ and the folding function are point-free.
myOr :: [Bool] -> Bool
myOr = foldr (||) False


-- Direct recursion not using â€˜||â€™.
myAny' :: (a -> Bool) -> [a] -> Bool
myAny' _ []     = False
myAny' f (x:xs) =
  if f x == True
  then True
  else myAny' f xs

-- Direct recursion using â€˜||â€™.
myAny'' :: (a -> Bool) -> [a] -> Bool
myAny'' _ []     = False
myAny'' f (x:xs) = f x || myAny' f xs

-- Fold, not point-free.
myAny''' :: (a -> Bool) -> [a] -> Bool
myAny''' f = foldr g False
  where g = (\x acc ->
               if f x == True
               then True
               else acc)


myAny :: (a -> Bool) -> [a] -> Bool
myAny f = foldr (||) False . map f



myElem :: Eq a => a -> [a] -> Bool
myElem _ [] = False
myElem e xs = myAny (== e) xs


myEl :: Eq a => a -> [a] -> Bool
myEl e = foldr (||) False . map (== e)

myEl' :: Eq a => a -> [a] -> Bool
myEl' e = foldr (\x acc -> acc || x == e) False


myRev :: [a] -> [a]
myRev = foldr (\x acc -> acc ++ [x]) []

myRev' :: [a] -> [a]
myRev' = foldl (flip (:)) []


myMap :: (a -> b) -> [a] -> [b]
myMap f = foldr (\x acc -> f x : acc) []


myFilter :: (a -> Bool) -> [a] -> [a]
myFilter f = foldr (\x acc ->
                      case f x of
                        True -> x : acc
                        False -> acc) []

squinsh :: [[a]] -> [a]
squinsh = foldr (\xs acc -> xs ++ acc) []


-- Why â€˜(a -> [b])â€™ instead of â€˜(a -> b)â€™?
squinshMap :: (a -> [b]) -> [a] -> [b]
squinshMap f = foldr (\x acc -> f x ++ acc) []
--
-- Î»> squinshMap (flip (:) []) [1..3]
-- [1,2,3]
--

squinshMap' :: (a -> [b]) -> [a] -> [b]
squinshMap' f = foldr ((++) . f) []

squinshAgain :: [[a]] -> [a]
squinshAgain = squinshMap id


myMaximumBy :: (a -> a -> Ordering) -> [a] -> a
myMaximumBy p xs = foldr (\x acc ->
                          if p x acc == GT
                          then x
                          else acc) (last xs) xs


myMininumBy :: (a -> a -> Ordering) -> [a] -> a
myMininumBy p xs = foldr (\x acc ->
                            if p x acc == LT
                            then x
                            else acc) (last xs) xs
```

### The End
